theories/rec_lang.v
@@ -1,0 +1,718 @@
+Require Import refframe.base.
+Require Import stdpp.strings.
+Require Import stdpp.propset.
+Require Import refframe.module.
+
+Import version7.
+
+
+
+(*
+
+
+some C:
+
+high-level spec -> events: system calls
+   ^
+   |  refines
+   |
+assembly code   -> events: system calls
+
+*)
+
+
+
+
+
+
+
+
+
+
+
+
+
+
+
+
+
+
+
+
+(*** stuff to move *)
+Definition state_set_refines {EV} (mimpl mspec : module EV) (σi : mimpl.(m_state)) (σs : propset mspec.(m_state)) : Prop :=
+  ∀ κs σi2, has_trace mimpl σi κs σi2 → ∃ σs1 σs2, σs1 ∈ σs ∧ has_trace mspec σs1 κs σs2.
+
+Lemma inv_set_implies_refines {EV} (m1 m2 : module EV) (inv : m1.(m_state) → propset m2.(m_state) → Prop):
+  inv m1.(m_initial) {[ m2.(m_initial) ]} →
+  (∀ σi σs, inv σi σs → ∃ σ, σ ∈ σs) →
+  (∀ σi σs, inv σi σs → m1.(m_is_ub) σi → ∃ σs1 σs2, σs1 ∈ σs ∧ has_trace m2 σs1 [Ub] σs2) →
+  (∀ σi1 σs1 σi2 e, inv σi1 σs1 → m1.(m_step) σi1 e σi2 →
+      ∃ σs2, inv σi2 σs2 ∧ σs2 ⊆ {[ σ2 | ∃ σ1, σ1 ∈ σs1 ∧ has_trace m2 σ1 (option_list (Vis <$> e)) σ2 ]}) →
+  refines m1 m2.
+Proof.
+  move => Hinvinit Hinvnonempty Hinvsafe Hinvstep.
+  constructor => // κs σi2.
+  move: m1.(m_initial) Hinvinit => σi1 Hinv Hsteps.
+  have : (∃ σs1 σs2, σs1 ∈ ({[m_initial m2]} : propset _) ∧ has_trace m2 σs1 κs σs2); last set_solver.
+  move: {[ m2.(m_initial) ]} Hinv => σs1 Hinv.
+  elim: Hsteps σs1 Hinv => {σi1 σi2 κs}.
+  - move => ? ? /Hinvnonempty [??].  eexists _, _. split => //. by apply: TraceEnd.
+  - move => σi1 σi2 σi3 κ κs Hstep Hsteps IH σs1 Hinv.
+    have [σs2 [Hinv2 Hsub]]:= Hinvstep _ _ _ _ Hinv Hstep.
+    have [σs3 [σs4 [Hin ?]]]:= IH _ Hinv2.
+    have [σ1 [??]]:= Hsub _ Hin.
+    eexists _, _. split => //. by apply: has_trace_trans.
+    (* case: (Hinvstep _ _ _ _ Hinv Hstep) => [|[σs2 [Hinv2 ?]]]. { *)
+    (*   case => Hub; [|eexists _; by apply: TraceUbRefl]. *)
+    (*   have [? /has_trace_ub_inv[σs2[??]]]:= Hinvsafe _ _ Hinv Hub. *)
+    (*   eexists σs2. apply: (has_trace_trans []); [ done |]. by apply: TraceUb. *)
+    (* } *)
+    (* case: (IH _ Hinv2) => ? ?. *)
+    (* eexists. by apply: has_trace_trans. *)
+  - move => ??? /Hinvsafe Hs σs Hinv.
+    have [? [? [? /has_trace_ub_inv[σs2[??]]]]]:= Hs _ Hinv.
+    eexists _, _. split => //. apply: (has_trace_trans []); [ done |]. by apply: TraceUbRefl.
+Qed.
+
+Lemma state_set_refines_initial {EV} (m1 m2 : module EV):
+  refines m1 m2 →
+  state_set_refines m1 m2 (m_initial m1) {[m_initial m2]}.
+Proof. move => [Hr] ?? /Hr[??]. naive_solver. Qed.
+
+Lemma state_set_refines_step {EV} (m1 m2 : module EV) σi1 σs1 σi2 e:
+  state_set_refines m1 m2 σi1 σs1 →
+  m1.(m_step) σi1 e σi2 →
+  state_set_refines m1 m2 σi2 {[ σ2 | ∃ σ1, σ1 ∈ σs1 ∧ has_trace m2 σ1 (option_list (Vis <$> e)) σ2 ]}.
+Proof.
+  move => Hinv Hstep κs σi3 Hκs.
+  have [|? [? [? /has_trace_app_inv[?[??]]]]]:= Hinv (option_list (Vis <$> e) ++ κs) σi3.
+  { by apply: TraceStep. }
+  set_solver.
+Qed.
+
+Lemma state_set_refines_step_None {EV} (m1 m2 : module EV) σi1 σs1 σi2:
+  state_set_refines m1 m2 σi1 σs1 →
+  m1.(m_step) σi1 None σi2 →
+  state_set_refines m1 m2 σi2 σs1.
+Proof.
+  move => Hinv Hstep κs σi3 Hκs.
+  have [|? [? [? ?]]]:= Hinv κs σi3.
+  { by apply: TraceStepNone. }
+  set_solver.
+Qed.
+
+Lemma state_set_refines_non_empty {EV} (m1 m2 : module EV) σi σs:
+  state_set_refines m1 m2 σi σs → ∃ σ, σ ∈ σs.
+Proof.
+  move => Hs.
+  have [|?[?[??]]]:= Hs [] σi. by apply: TraceEnd.
+  naive_solver.
+Qed.
+
+Lemma state_set_refines_ub {EV} (m1 m2 : module EV) σi σs:
+  state_set_refines m1 m2 σi σs →
+  m1.(m_is_ub) σi →
+  ∃ σ σ', σ ∈ σs ∧ has_trace m2 σ [Ub] σ'.
+Proof. move => Hs Hub. apply: Hs. by apply: TraceUbRefl. Qed.
+
+Lemma refines_implies_inv_set {EV} (m1 m2 : module EV):
+  refines m1 m2 →
+  ∃ (inv : m1.(m_state) → propset m2.(m_state) → Prop),
+  inv m1.(m_initial) {[ m2.(m_initial) ]} ∧
+  (∀ σi σs, inv σi σs → ∃ σ, σ ∈ σs) ∧
+  (∀ σi σs, inv σi σs → m1.(m_is_ub) σi → ∃ σs1 σs2, σs1 ∈ σs ∧ has_trace m2 σs1 [Ub] σs2) ∧
+  (∀ σi1 σs1 σi2 e, inv σi1 σs1 → m1.(m_step) σi1 e σi2 →
+      ∃ σs2, inv σi2 σs2 ∧ σs2 ⊆ {[ σ2 | ∃ σ1, σ1 ∈ σs1 ∧ has_trace m2 σ1 (option_list (Vis <$> e)) σ2 ]}).
+Proof.
+  move => Href.
+  eexists (state_set_refines m1 m2).
+  split_and!.
+  - by apply: state_set_refines_initial.
+  - by apply: state_set_refines_non_empty.
+  - move => σi σs Hinv Hub. by apply: state_set_refines_ub.
+  - move => σi1 σs1 σi2 e Hinv Hstep.
+    eexists _. split_and!; last reflexivity.
+    by apply: state_set_refines_step.
+Qed.
+
+(* Lemma state_refines_ub {EV} (m1 m2 : module EV) σ1 σ2 : *)
+(*   state_refines m1 m2 σ1 σ2 → *)
+(*   m1.(m_is_ub) σ1 → ∃ σ2', has_trace m2 σ2 [] σ2' ∧ m2.(m_is_ub) σ2'. *)
+(* Proof. *)
+(*   move => Hs Hub. *)
+(*   have [|? /has_trace_ub_inv [?[??]]]:= Hs [Ub] σ1. { by apply: TraceUbRefl. } *)
+(*   naive_solver. *)
+(* Qed. *)
+
+(* Lemma state_refines_step_Some {EV} (m1 m2 : module EV) σ1 σ2 e σ1': *)
+(*   state_refines m1 m2 σ1 σ2 → *)
+(*   m1.(m_step) σ1 (Some e) σ1' → *)
+(*   ∃ σ2', has_trace m2 σ2 [Vis e] σ2' ∧ state_refines m1 m2 σ1' σ2'. *)
+(* Proof. *)
+(*   move => Hs Hub. *)
+(*   have [|? /(has_trace_cons_inv _ _)[?[?[? Hor]]]]:= Hs [Vis e] σ1'. { *)
+(*     apply: TraceStepSome; [| by apply:TraceEnd ]. done. *)
+(*   } *)
+(*   case: Hor => [?|[??]]. *)
+(*   - eexists _. split. { apply: (has_trace_trans []) => //. by apply: TraceUbRefl. } *)
+(*     admit. *)
+(*   - *)
+(*     (* eexists _. split. { apply: (has_trace_trans []) => //. apply: TraceStepSome. done. apply: TraceEnd. } *) *)
+(*     (* move => ???. eexists _. *) *)
+(* (* Qed. *) *)
+(* Abort. *)
+
+(* Lemma state_refines_step {EV} (m1 m2 : module EV) σ1 σ2 e σ1': *)
+(*   state_refines m1 m2 σ1 σ2 → *)
+(*   m1.(m_step) σ1 e σ1' → *)
+(*   ∃ σ2', has_trace m2 σ2 (option_list (Vis <$> e)) σ2' ∧ state_refines m1 m2 σ1' σ2'. *)
+(* Proof. *)
+(* Admitted. *)
+
+
+Module rec.
+Definition fn_name := string.
+Definition var_name := string.
+
+Inductive binop : Set :=
+| AddOp.
+
+Inductive cmp : Set :=
+| EqCmp.
+
+Inductive expr : Set :=
+| Var (v : var_name)
+| Const (n : Z)
+| BinOp (v1 : var_name) (o : binop) (v2 : var_name)
+| If (v1 : var_name) (c : cmp) (v2 : var_name) (e1 e2 : expr)
+| LetE (v : var_name) (e1 e2 : expr)
+| Call (f : fn_name) (args : list var_name)
+.
+Record fndef : Type := {
+  fd_args : list var_name;
+  fd_body : expr;
+}.
+Record cont := {
+  c_var : var_name;
+  c_env : gmap var_name Z;
+  c_expr : expr;
+}.
+
+(*
+                          -----------
+                         v           \
+  WaitingForCall -> Running -> WaitingForReturn
+                       |
+                       v
+                    Finished
+
+
+                          -----------
+                         v           \          Push
+  WaitingForCall -> Running -> WaitingForReturn --> WaitingForCall
+                       |
+                       v
+                    Finished
+*)
+Inductive state_kind : Set :=
+| Running (e : expr) | WaitingForCall | WaitingForReturn | Finished | Stuck.
+Record state := {
+  st_exp : state_kind;
+  st_env : gmap var_name Z;
+  st_conts : list cont;
+  st_fns : gmap fn_name fndef;
+}.
+Inductive rec_event : Type :=
+| RecvCallEvt (fn : string) (args: list Z) | RecvRetEvt (ret: Z)
+| CallEvt (fn : string) (args: list Z) | DoneEvt (ret: Z).
+
+Inductive step : state → option rec_event → state → Prop :=
+(* Internal steps *)
+| VarStep v ρ fns n cs:
+    ρ !! v = Some n →
+    step {| st_exp := Running (Var v); st_env := ρ; st_conts := cs; st_fns := fns |}
+         None
+         {| st_exp := Running (Const n); st_env := ρ; st_conts := cs; st_fns := fns |}
+| BinOpStep v1 v2 o ρ fns n1 n2 nr cs:
+    ρ !! v1 = Some n1 →
+    ρ !! v2 = Some n2 →
+    nr = match o with | AddOp => n1 + n2 end%Z →
+    step {| st_exp := Running (BinOp v1 o v2); st_env := ρ; st_conts := cs; st_fns := fns |}
+         None
+         {| st_exp := Running (Const nr); st_env := ρ; st_conts := cs; st_fns := fns |}
+| IfStep v1 v2 c ρ fns n1 n2 b e1 e2 cs:
+    ρ !! v1 = Some n1 →
+    ρ !! v2 = Some n2 →
+    b = match c with | EqOp => bool_decide (n1 = n2) end →
+    step {| st_exp := Running (If v1 c v2 e1 e2); st_env := ρ; st_conts := cs; st_fns := fns |}
+         None
+         {| st_exp := Running (if b then e1 else e2); st_env := ρ; st_conts := cs; st_fns := fns |}
+| LetStep v e1 e2 ρ fns cs:
+    step {| st_exp := Running (LetE v e1 e2); st_env := ρ; st_conts := cs; st_fns := fns |}
+         None
+         {| st_exp := Running e1; st_env := ρ; st_conts := {|c_var := v; c_env := ρ; c_expr := e2|} :: cs; st_fns := fns |}
+| CallInternalStep f vas ρ cs fns nas fn:
+    Forall2 (λ n v, ρ !! n = Some v) vas nas →
+    fns !! f = Some fn →
+    length vas = length fn.(fd_args) →
+    step {| st_exp := Running (Call f vas); st_env := ρ; st_conts := cs; st_fns := fns |}
+         None
+         {| st_exp := Running fn.(fd_body); st_env := list_to_map (zip fn.(fd_args) nas); st_conts := cs; st_fns := fns |}
+(* External Calls *)
+| CallExternalStep f vas ρ cs fns nas:
+    Forall2 (λ n v, ρ !! n = Some v) vas nas →
+    fns !! f = None →
+    step {| st_exp := Running (Call f vas); st_env := ρ; st_conts := cs; st_fns := fns |}
+         (Some (CallEvt f nas))
+         {| st_exp := WaitingForReturn; st_env := ρ; st_conts := cs; st_fns := fns |}
+| RecvReturnStep ρ cs fns n:
+    step {| st_exp := WaitingForReturn; st_env := ρ; st_conts := cs; st_fns := fns |}
+         (Some (RecvRetEvt n))
+         {| st_exp := Running (Const n); st_env := ρ; st_conts := cs; st_fns := fns |}
+| RecvCallStep ρ cs fns nas σ fn f:
+    fns !! f = Some fn →
+    σ = (if bool_decide (length nas = length fn.(fd_args)) then Running fn.(fd_body) else Stuck) →
+    step {| st_exp := WaitingForCall; st_env := ρ; st_conts := cs; st_fns := fns |}
+         (Some (RecvCallEvt f nas))
+         {| st_exp := σ; st_env := list_to_map (zip fn.(fd_args) nas); st_conts := cs; st_fns := fns |}
+(* Const steps *)
+| ConstConsStep n c ρ fns cs:
+    step {| st_exp := Running (Const n); st_env := ρ; st_conts := c::cs; st_fns := fns |}
+         None
+         {| st_exp := Running c.(c_expr); st_env := <[c.(c_var) := n]>c.(c_env); st_conts := cs; st_fns := fns |}
+| ConstNilStep n ρ fns:
+    step {| st_exp := Running (Const n); st_env := ρ; st_conts := []; st_fns := fns |}
+         (Some (DoneEvt n))
+         {| st_exp := Finished; st_env := ρ; st_conts := []; st_fns := fns |}
+.
+
+Definition rec_fns := gmap string fndef.
+
+Definition is_ub (σ : state) : Prop :=
+  ¬ (σ.(st_exp) = Finished ∨ ∃ e σ', step σ e σ').
+
+Definition initial_state (fns: rec_fns) : state :=
+  {|
+    st_exp := WaitingForCall;
+    st_conts := [];
+    st_fns := fns;
+    st_env := ∅;
+  |}.
+
+Definition rec_module (fns: rec_fns) : module rec_event := {|
+  m_state := state;
+  m_initial := initial_state fns;
+  m_step := step;
+  m_is_ub := is_ub;
+|}.
+
+Definition rec_link (fns1 fns2 : rec_fns) : rec_fns := fns1 ∪ fns2.
+
+Definition ctx_refines (fnsi fnss : rec_fns) :=
+  ∀ C, refines (rec_module (rec_link fnsi C)) (rec_module (rec_link fnss C)).
+
+Definition ctx_equiv (fnsi fnss : rec_fns) :=
+  ctx_refines fnsi fnss ∧ ctx_refines fnss fnsi.
+
+
+(*** Call module *)
+Record call_module_info (EV : Type) := {
+  (* TODO: Should these go into Prop instead? That would be more
+  expressive, but call_step already requires these properties to be
+  basically decidable, so it probably does not make a difference in
+  practice and this version is nicer to use. *)
+  cmi_final : EV → bool;
+  cmi_waiting : EV → bool;
+}.
+Arguments cmi_final {_}.
+Arguments cmi_waiting {_}.
+
+Record call_state {EV} (m : module EV) := {
+  cs_stack : list m.(m_state);
+  cs_waiting : bool;
+}.
+Arguments cs_stack {_ _}.
+Arguments cs_waiting {_ _}.
+
+Inductive call_step {EV} (m : module EV) (i : call_module_info EV) : (call_state m) → option EV → (call_state m) → Prop :=
+| CStep σ σs σ' e w cs:
+    m.(m_step) σ e σ' →
+    cs = (if default false (i.(cmi_final) <$> e) then [] else [σ']) ++ σs →
+    call_step m i {| cs_stack := (σ :: σs); cs_waiting := w |}
+              e {| cs_stack := cs; cs_waiting := default w (i.(cmi_waiting) <$> e) |}
+| CWaiting σs:
+    call_step m i {| cs_stack := σs; cs_waiting := true |}
+              None {| cs_stack := m.(m_initial) :: σs; cs_waiting := false |}
+.
+
+Definition call_module {EV} (m : module EV) (i : call_module_info EV) : module EV := {|
+  m_state := call_state m;
+  m_initial := {| cs_stack := []; cs_waiting := true |};
+  m_step := call_step m i;
+  m_is_ub σ := default False (m.(m_is_ub) <$> head σ.(cs_stack));
+|}.
+
+Definition call_module_refines_inv {EV} (m1 m2 : module EV) (i : call_module_info EV) (σ1 : (call_module m1 i).(m_state)) (sσ2 : propset (call_module m2 i).(m_state)) : Prop :=
+  ∃ Ts, Forall2 (state_set_refines m1 m2) σ1.(cs_stack) Ts
+    ∧ sσ2 ≡ {[ σ2 | σ1.(cs_waiting) = σ2.(cs_waiting) ∧ Forall2 elem_of σ2.(cs_stack) Ts ]}.
+
+  (* ∀ σ2, σ2 ∈ sσ2 → ( *)
+  (*         (* Forall2 elem_of σ2.(cs_stack) (PropSet <$> (state_refines m1 m2 <$> σ1.(cs_stack)))). *) *)
+
+  (* Forall2 (state_refines m1 m2) σ1.(cs_stack) σ2.(cs_stack) ∧ *)
+  (* σ1.(cs_waiting) = σ2.(cs_waiting)). *)
+
+Lemma call_empty_steps {EV} (m : module EV) i σ σ' w σs:
+  has_trace m σ [] σ' →
+  has_trace (call_module m i) {| cs_stack := σ :: σs; cs_waiting := w |} []
+            {| cs_stack := σ' :: σs; cs_waiting := w |}.
+Proof.
+  move Hκ: ([]) => κ Hsteps.
+  elim: Hsteps Hκ.
+  - move => ?. by econstructor.
+  - move => σ1 σ2 σ3 [?|] κs //= ?? IH ?. subst.
+    apply: TraceStepNone; [ | by apply: IH]. by apply: CStep.
+  - move => ?????. by apply: TraceUb => /=.
+Qed.
+
+Lemma state_set_refines_exists_Forall2 {EV} (m1 m2 : module EV) σ σs:
+  Forall2 (state_set_refines m1 m2) σ σs →
+  ∃ σs', Forall2 elem_of σs' σs.
+Proof.
+  elim. { eexists []. constructor. }
+  move => ???? /state_set_refines_non_empty[??] ? [??].
+  eexists. by constructor.
+Qed.
+
+Lemma call_module_refines {EV} (m1 m2 : module EV) (i : call_module_info EV) :
+  refines m1 m2 →
+  refines (call_module m1 i) (call_module m2 i).
+Proof.
+  move => Href.
+  apply (inv_set_implies_refines _ _ (call_module_refines_inv _ _ _)).
+  - eexists []. split_and!; [ by constructor |].
+    set_unfold; move => [??] /=. split; first naive_solver.
+    move => [-> Hall]. inversion Hall. naive_solver.
+  - move => [??] ? [Ts [/state_set_refines_exists_Forall2 [??] Hσs]].
+    eexists (Build_call_state _ _ _ _). by rewrite {}Hσs.
+  - move => [csi wi] σs /= [Ts [Hall Hσs]] Hub. destruct csi => //; simplify_eq/=.
+    move: Hall => /(Forall2_cons_inv_l _ _ _)[? [? [ /state_set_refines_ub [//|σ1 [σ1' [? Hub2]]] [/state_set_refines_exists_Forall2[??] ?]]]] /=. subst.
+    move: Hub2 => /has_trace_ub_inv[? [??]].
+    eexists (Build_call_state _ _ _ _), _. rewrite {}Hσs. split.
+    { split => //. by constructor. }
+    apply: (has_trace_trans []); [ by apply: call_empty_steps|].
+    by apply: TraceUbRefl.
+  - move => [csi wi] σs [csi2 wi2] e [Ts [Hall Hσs]] /= Hstep.
+    invert_all @call_step.
+    + revert select (m_step _ _ _ _) => Hstep.
+      move: Hall => /(Forall2_cons_inv_l _ _ _)[? [Ts' [Hs[??]]]]. subst.
+      destruct e as [e|] => /=. 2: {
+        eexists σs. split.
+        - eexists _. split; [|set_solver].
+          constructor => //. by apply: state_set_refines_step_None.
+        - move => σ1 ?. eexists σ1. split => //. apply: TraceEnd.
+      }
+      eexists _. split. {
+        eexists ((if cmi_final i e then [] else [_]) ++ Ts').
+        split => //.
+        apply: Forall2_app => //.
+        case_match. constructor. constructor; [|by constructor].
+          by apply: state_set_refines_step.
+      }
+      move => /= [??] [? Hall]. simplify_eq/=.
+      case_match; simplify_eq/=.
+      * have /state_set_refines_non_empty[σa [σb /= [? Ht]]] := state_set_refines_step _ _ _ _ _ _ Hs Hstep.
+        eexists (Build_call_state _ _ _ _). rewrite {}Hσs.
+        split. { split => //. apply: Forall2_cons => //. }
+        move: Ht => /(has_trace_cons_inv _ _ _)[? [? [? Hor]]].
+        apply: (has_trace_trans []); [ by apply: call_empty_steps|].
+        case: Hor => [?|[??]]; [by apply: TraceUb|].
+        apply: TraceStepSome; [|by apply: TraceEnd].
+        apply: CStep => //. case_match => //. simplify_eq/=. congruence.
+      * move: Hall => /(Forall2_cons_inv_r _ _ _ _)[σa [Ts [[σb [? Ht]][??]]]].
+        simplify_eq.
+        eexists (Build_call_state _ _ _ _). rewrite {}Hσs.
+        split. { split => //. apply: Forall2_cons => //. }
+        move: Ht => /(has_trace_cons_inv _ _ _)[? [? [? Hor]]].
+        apply: (has_trace_trans []); [ by apply: call_empty_steps|].
+        case: Hor => [?|[??]]; [by apply: TraceUb|].
+        apply: TraceStepSome. { by apply: CStep. }
+        case_match => //; simplify_eq/=; try congruence.
+        by apply: call_empty_steps.
+    + eexists _. split_and!. {
+        eexists _. split; [|done]. apply: Forall2_cons; [|done].
+          by apply: state_set_refines_initial.
+      }
+      move => [??] [? /(Forall2_cons_inv_r _ _ _ _) [? [?[? [??]]]]]. simplify_eq/=.
+      eexists (Build_call_state _ _ _ _). rewrite Hσs.
+      split. { split => //. }
+      apply: TraceStepNone; [|by apply: TraceEnd].
+      set_unfold; subst. by apply CWaiting.
+      (* 3: { move => ??. eexists _. apply: TraceStepNone; [|by apply: TraceEnd]. apply: CWaiting. } *)
+      (* split => //. constructor => //. by apply: ref_subset. *)
+Qed.
+
+Definition call_module_link_inv {EV} (m1 m2 m3 : module EV) (i : call_module_info EV) (M : link_mediator EV EV EV) (σ1 : (call_module m1 i).(m_state)) (σ2 : (call_module m2 i).(m_state)) (σ3 : (call_module m3 i).(m_state)) (σm : M.(lm_state)) : Prop :=
+  True.
+
+Lemma call_module_refines_link {EV} (m1 m2 m3 : module EV) (i : call_module_info EV) M :
+  refines_equiv (call_module m1 i) (link (call_module m2 i) (call_module m3 i) M).
+Proof.
+  apply (inv_implies_refines_equiv _ (link _ _ _) (curry ∘ curry ∘ (call_module_link_inv _ _ _ _ _))).
+  - done.
+  - admit.
+  - admit.
+  - move => [cs1 ws1] [[[cs2 ws2] [cs3 ws3]] σm] [??] ?/= ? ?.
+    invert_all @call_step.
+    * right.
+      admit.
+    * admit.
+  - move => [cs1 ws1] [[[cs2 ws2] [cs3 ws3]] σm] [??] ?/= ? ?.
+    admit.
+    (* invert_all @link_step. *)
+Admitted.
+
+
+(*** rec linking *)
+Definition rec_cmi : call_module_info rec_event := {|
+  cmi_final e := if e is DoneEvt _ then true else false;
+  cmi_waiting e := if e is CallEvt _ _ then true else false;
+|}.
+
+Definition rec_link_mediator (fns1 fns2 : gset string) : link_mediator rec_event rec_event rec_event.
+Admitted.
+
+Lemma rec_link_ok fns1 fns2:
+  fns1 ##ₘ fns2 →
+  refines_equiv (call_module (rec_module (rec_link fns1 fns2)) rec_cmi)
+          (link (call_module (rec_module fns1) rec_cmi) (call_module (rec_module fns2) rec_cmi)
+                (rec_link_mediator (dom _ fns1) (dom _ fns2))).
+Proof.
+  move => ?.
+  apply call_module_refines_link.
+Admitted.
+
+Definition rec_call_mediator : link_mediator rec_event Empty_set rec_event.
+Admitted.
+
+Lemma rec_refines_call fns:
+  refines_equiv (rec_module fns) (link (call_module (rec_module fns) rec_cmi) ∅ rec_call_mediator).
+Proof.
+Admitted.
+
+Lemma refines_implies_rec_ctx_refines fnsi fnss :
+  dom (gset string) fnsi = dom (gset string) fnss →
+  refines (rec_module fnsi) (rec_module fnss) →
+  ctx_refines fnsi fnss.
+Proof.
+  move => Hdom Href C.
+  rewrite /rec_link map_difference_union_r (map_difference_union_r fnss).
+  apply: refines_vertical. { apply rec_refines_call. }
+  apply: refines_vertical. 2: { apply rec_refines_call. }
+  apply: refines_horizontal. 2: { apply refines_reflexive. }
+
+  apply: refines_vertical. { apply rec_link_ok. apply: map_disjoint_difference_r'. }
+  apply: refines_vertical. 2: { apply rec_link_ok. apply: map_disjoint_difference_r'. }
+  rewrite !dom_difference_L !Hdom.
+  apply: refines_horizontal.
+  - apply: call_module_refines. apply: Href.
+  - rewrite (map_difference_eq_dom_L _ _ _ Hdom).
+    apply refines_reflexive.
+Qed.
+
+Lemma refines_equiv_implies_rec_ctx_equiv fnsi fnss :
+  dom (gset string) fnsi = dom (gset string) fnss →
+  refines_equiv (rec_module fnsi) (rec_module fnss) →
+  ctx_equiv fnsi fnss.
+Proof. move => ? [??]. split; by apply refines_implies_rec_ctx_refines. Qed.
+
+Lemma refines_equiv_equiv_rec_ctx_equiv fnsi fnss :
+  dom (gset string) fnsi = dom (gset string) fnss →
+  refines_equiv (rec_module fnsi) (rec_module fnss) ↔
+  ctx_equiv fnsi fnss.
+Proof.
+  move => ?. split; [by apply: refines_equiv_implies_rec_ctx_equiv|].
+  move => [Hi Hs].
+  pose proof (Hi ∅) as Hi.
+  pose proof (Hs ∅) as Hs.
+  rewrite /rec_link !right_id_L in Hi Hs.
+  done.
+Qed.
+
+(*** Test module *)
+Module test.
+  Local Open Scope Z_scope.
+
+  Definition add1 : fndef := {|
+    fd_args := ["a"];
+    fd_body := LetE "1" (Const 1) $ BinOp "a" AddOp "1";
+  |}.
+
+  Definition add1_cumbersome : fndef := {|
+    fd_args := ["a"];
+    fd_body :=
+      LetE "2" (Const 2) $
+      LetE "-1" (Const (-1)) $
+      LetE "res" (BinOp "a" AddOp "2") $
+      (BinOp "res" AddOp "-1") ;
+  |}.
+
+  Definition ret2 : fndef := {|
+    fd_args := [];
+    fd_body := Const 2;
+  |}.
+
+  Definition ret2_call : fndef := {|
+    fd_args := [];
+    fd_body :=
+      LetE "1" (Const 1) $
+      Call "add1" ["1"]
+  |}.
+
+  Definition const_prop_pre : fndef := {|
+    fd_args := [];
+    fd_body :=
+      LetE "2" (Const 2) $
+      LetE "u" (Call "unknown" []) $
+      BinOp "u" AddOp "2"
+  |}.
+
+  Definition const_prop_post : fndef := {|
+    fd_args := [];
+    fd_body :=
+      LetE "u" (Call "unknown" []) $
+      LetE "2" (Const 2) $
+      BinOp "u" AddOp "2"
+  |}.
+
+  Lemma add1_refines_cumbersome add1_name :
+    refines (rec_module {[ add1_name := add1 ]}) (rec_module {[ add1_name := add1_cumbersome ]}).
+  Proof.
+    apply: wp_implies_refines => n.
+    constructor. split. { apply. right. eexists _, _. econstructor => //. by apply: lookup_insert. }
+    move => ? ? ? ? ?. inv_step. simplify_map_eq.
+    destruct (decide (length nas = 1%nat)). 2: {
+      eexists _. left. apply: TraceStepSome. { econstructor => //. apply: lookup_insert. }
+      apply: TraceUbRefl => /=. case_bool_decide => //.
+      move => [?//|[? [??]]]. invert_all step.
+    }
+    eexists _. right. split. {
+      apply: TraceStepSome; [|by apply: TraceEnd].
+      econstructor => //. by apply: lookup_insert.
+    }
+    simpl. case_bool_decide => //.
+    destruct nas as [|n [|]] => //.
+
+    constructor. split. { apply. right. eexists _, _. by econstructor. }
+    move => ?????. inv_step.
+    eexists. right. split. { apply: TraceEnd. }
+
+    constructor. split. { apply. right. eexists _, _. by econstructor. }
+    move => ?????. inv_step.
+    eexists. right. split. { apply: TraceEnd. }
+
+    constructor. split. { apply. right. eexists _, _. by econstructor. }
+    move => ?????. inv_step.
+    eexists. right. split. { apply: TraceEnd. }
+
+    constructor. split. { apply. right. eexists _, _. by econstructor. }
+    move => ?????. inv_step. simplify_map_eq.
+    eexists. right. split. {
+      simpl. apply: TraceStepNone. { by econstructor. }
+      simpl. apply: TraceStepNone. { by econstructor. }
+      simpl. apply: TraceStepNone. { by econstructor. }
+      simpl. apply: TraceStepNone. { by econstructor. }
+      simpl. apply: TraceStepNone. { by econstructor. }
+      simpl. apply: TraceStepNone. { by econstructor. }
+      simpl. apply: TraceStepNone. { by econstructor. }
+      simpl. apply: TraceStepNone. { by econstructor. }
+      simpl. apply: TraceStepSome. {
+        have -> : (n1 + 2 + -1) = n1 + 1 by lia.
+        by econstructor.
+      }
+      apply: TraceEnd.
+    }
+
+    constructor. split. { apply. by left. }
+    move => ?????. inv_step.
+    Unshelve.
+    apply: inhabitant.
+  Qed.
+
+  Lemma ret2_refines_call :
+    refines (rec_module (<[ "add1" := add1]> {["ret2" := ret2 ]})) (rec_module (<[ "add1" := add1]> {["ret2" := ret2_call ]})).
+  Proof.
+    apply: wp_implies_refines => n.
+  Admitted.
+
+  Lemma const_prop_post_refines_pre  :
+    refines (rec_module {[ "cp" := const_prop_post ]}) (rec_module {[ "cp" := const_prop_pre ]}).
+  Proof.
+    apply: wp_implies_refines => n.
+    constructor. split. { apply. right. eexists _, _. econstructor => //. by apply: lookup_insert. }
+    move => ? ? ? ? ?. inv_step. simplify_map_eq.
+    destruct (decide (length nas = 0%nat)). 2: {
+      eexists _. left. apply: TraceStepSome. { econstructor => //. }
+      apply: TraceUbRefl => /=. case_bool_decide => //.
+      move => [?//|[? [??]]]. invert_all step.
+    }
+    eexists _. right. split. {
+      apply: TraceStepSome; [|by apply: TraceEnd].
+      econstructor => //.
+    }
+    simpl. case_bool_decide => //.
+    destruct nas as [|n [|]] => //.
+
+    constructor. split. { apply. right. eexists _, _. by econstructor. }
+    move => ?????. inv_step.
+    eexists. right. split. { apply: TraceEnd. }
+
+    constructor. split. { apply. right. eexists _, _. by econstructor. }
+    move => ?????. inv_step.
+    revert select (Forall2 _ [] _) => /Forall2_nil_inv_l ->.
+    eexists. right. split. {
+      simpl. apply: TraceStepNone. { by econstructor. }
+      simpl. apply: TraceStepNone. { by econstructor. }
+      simpl. apply: TraceStepNone. { by econstructor. }
+      simpl. apply: TraceStepSome. { by econstructor. }
+      apply: TraceEnd.
+    }
+    constructor. split. { apply. right. eexists _, _. by econstructor. }
+    move => ?????. inv_step.
+    eexists. right. split. {
+      simpl. apply: TraceStepSome. { by econstructor. }
+      apply: TraceEnd.
+    }
+
+    constructor. split. { apply. right. eexists _, _. by econstructor. }
+    move => ?????. inv_step.
+    eexists. right. split. { apply: TraceEnd. }
+
+    constructor. split. { apply. right. eexists _, _. by econstructor. }
+    move => ?????. inv_step.
+    eexists. right. split. { apply: TraceEnd. }
+
+    constructor. split. { apply. right. eexists _, _. by econstructor. }
+    move => ?????. inv_step.
+    eexists. right. split. { apply: TraceEnd. }
+
+    constructor. split. { apply. right. eexists _, _. by econstructor. }
+    move => ?????. inv_step. simplify_map_eq.
+    eexists. right. split. { apply: TraceEnd. }
+
+    constructor. split. { apply. right. eexists _, _. by econstructor. }
+    move => ?????. inv_step.
+    eexists. right. split. {
+      simpl. apply: TraceStepNone. { by econstructor. }
+      simpl. apply: TraceStepNone. { by econstructor. }
+      simpl. apply: TraceStepSome. { by econstructor. }
+      apply: TraceEnd.
+    }
+
+    constructor. split. { apply. by left. }
+    move => ?????. inv_step.
+    Unshelve.
+    all: apply: inhabitant.
+  Qed.
+End rec.
